Progress

CellularAutomatas/proofs/cart_transducers.lean
@@ -60,3 +60,144 @@ theorem CArtTransducer.scan_temporal_independence [Alphabet α] [Alphabet Γ] (C
   simp
   rw [←List.map_take]
   rw [LCellAutomaton.scan_temporal_independence]
+
+
+
+
+
+
+
+
+namespace compress_by_3
+  variable [Alphabet α] [Alphabet β]
+
+  theorem compression1 (C: LCellAutomaton α):
+      ∃ (C': LCellAutomaton α) (f: C'.Q → Option (C.Q × C.Q × C.Q)),
+      ∀ w (t: ℕ) (p: ℤ),
+        f (C'.comp w t p) =
+          if p >= 0 ∧ t = 2 * p + 3
+          then
+            let i := (3 * p).natAbs;
+            some (C.comp w (i) 0, C.comp w (i + 1) 0, C.comp w (i + 2) 0)
+          else none
+          := by
+    sorry
+
+end compress_by_3
+
+
+
+namespace speedup_factor_k
+  variable [Alphabet α] [Alphabet β]
+
+  variable {Q: Type}
+  variable (k: ℕ) [NeZero k]
+
+  def compress (c: Config Q): Config (Fin k → Q) :=
+    fun p => fun j => c (p * k + j)
+
+  def decompress (c: Config (Fin k → Q)): Config Q :=
+    fun p => c (p / k) (Fin.intCast p)
+
+  lemma compress_decompress (c: Config Q):
+      decompress k (compress k c) = c := by
+        sorry
+
+  variable (C: CellAutomaton)
+
+  def Q' := Fin k → C.Q
+
+  def local_config (a b c: Q' k C): Config C.Q :=
+      fun p => if p <= -k then a (Fin.intCast 0) else
+        if p < 0 then a (Fin.intCast (p + k))
+        else if p < k then b (Fin.intCast p)
+        else c (Fin.intCast (p - k))
+
+  def to_local_config (c: Config (C.Q)): Q' k C := fun j => c j
+
+  def C': CellAutomaton := {
+    Q := Fin k → C.Q
+    δ := fun a b c =>
+      to_local_config k C (C.nextt (local_config k C (a) (b) (c)) k)
+  }
+
+
+
+  lemma compression_k_step (c: Config C.Q):
+      (C' k C).next (compress k c) = compress k (C.nextt c k) :=
+        sorry
+
+  theorem spec (c: Config C.Q):
+      ∀ t, (C' k C).nextt (compress k c) t = compress k (C.nextt c (k * t)) :=
+        sorry
+
+end speedup_factor_k
+
+
+
+namespace simulation
+  structure Params where
+    C_inr: CellAutomaton
+    C_ctl: CellAutomaton
+    f: C_ctl.Q → Option C_inr.Q
+
+  variable (e: Params)
+/-
+
+  structure Q1 where
+    state: e.C_ctl.Q
+    counter: Fin 3
+  deriving Inhabited, DecidableEq, Fintype
+
+  instance [Alphabet α] : Alphabet (Option α) := {}
+  instance : Alphabet (Q1 e) := {}
+
+  def C': CellAutomaton := {
+    Q := Option (Q1 e × e.C_inr.Q)
+    δ := fun a b c =>
+      match (a, b, c) with
+      | (some qa, some (qb, _), some qc) =>
+        if qb.counter = 2
+        then sorry
+        else none
+      | _ => none
+  }
+
+  variable (c_ctl: Config e.C_ctl.Q)
+  variable (c_inr: Config e.C_inr.Q)
+  variable (h_CM: ∀ (t: ℕ) (p: ℤ),
+    e.f (e.C_ctl.nextt c_ctl t p) =
+      if t = 3 + 2 * p.natAbs then some (c_inr p)
+      else none
+  )
+
+
+  def to_C'Q: e.C_ctl.Q → (C' e).Q := sorry
+  def to_CinrQ: (C' e).Q → e.C_inr.Q := sorry
+
+  theorem spec: ∀ (t: ℕ) (p: ℤ),
+    let c' := (to_C'Q e) ∘ c_ctl
+    let proj := to_CinrQ e;
+    let C' := C' e
+    proj (C'.nextt c' (3 + 3 * t) 0) = e.C_inr.nextt c_inr t 0 := by
+      sorry
+-/
+end simulation
+
+
+
+
+
+
+
+
+
+def CArtTransducer.compose [Alphabet α] [Alphabet β] [Alphabet γ] (t1: CArtTransducer β γ) (t2: CArtTransducer α β):
+    CArtTransducer α γ :=
+  sorry
+
+def CArtTransducer.compose_spec [Alphabet α] [Alphabet β] [Alphabet γ]
+    {t1: CArtTransducer β γ} {t2: CArtTransducer α β}:
+    (CArtTransducer.compose t1 t2).advice.f =
+      t1.advice.f ∘ t2.advice.f := by
+        sorry
