CellularAutomatas/proofs/finite_state_transducers.lean
@@ -1,84 +1,319 @@
 import CellularAutomatas.defs
 import Mathlib.Data.List.Basic
+import Mathlib.Data.List.TakeDrop
+import Mathlib.Tactic.Linarith
 
-
-def id_transducer (Q) [Alphabet Q]: FiniteStateTransducer Q Q := {
-  Q := Q
-  δ := fun _ a => a
-  q0 := default
-  f := id
-}
-
-@[simp]
-lemma id_transducer_scanr_eq [Alphabet Q]:
-  (id_transducer Q).scanr = id := by
-  funext w
-  simp [FiniteStateTransducer.scanr, FiniteStateTransducer.scanr_q]
-  induction w with
-  | nil => rfl
-  | cons a w ih =>
-    simp [FiniteStateTransducer.scanr_step]
-    rw [ih]
-    cases w <;> simp [id_transducer]
-
-@[simp]
-lemma id_transducer_advice_eq [Alphabet Q]:
-  (id_transducer Q).advice.f = id := by
-  simp [FiniteStateTransducer.advice]
-  rfl
 
 
 def FiniteStateTransducer.map_output [Alphabet α] [Alphabet β] [Alphabet γ]
-    {M: FiniteStateTransducer α β} (g: β → γ): FiniteStateTransducer α γ := {
+    (M: FiniteStateTransducer α β) (g: β → γ): FiniteStateTransducer α γ := {
   Q := M.Q
   δ := M.δ
   q0 := M.q0
   f := g ∘ M.f
 }
 
+@[simp]
+lemma FiniteStateTransducer.map_output_spec [Alphabet α] [Alphabet β] [Alphabet γ] {M: FiniteStateTransducer α β} {g: β → γ}:
+    (M.map_output g).scanr = (List.map g) ∘ M.scanr := by
+      sorry
+
 
 namespace FiniteStateTransducer
+  section
 
-  variable {α β : Type} {M: FiniteStateTransducer α β}
+    variable {α β : Type} {M: FiniteStateTransducer α β}
 
-  lemma scanr_foldr_state (p: Word α) (q: M.Q) (tail: List β):
-      (p.foldr M.scanr_step (q, tail)).fst = M.scanr_reduce_q q p := by
-    induction p generalizing q tail with
-    | nil => simp [scanr_reduce_q]
-    | cons a p' ih =>
-      simp [scanr_step, scanr_reduce_q]
-      rw [ih]
+    lemma scanr_foldr_state (p: Word α) (q: M.Q) (tail: List β):
+        (p.foldr M.scanr_step (q, tail)).fst = M.scanr_reduce_q q p := by
+      induction p generalizing q tail with
+      | nil => simp [scanr_reduce_q]
+      | cons a p' ih =>
+        simp [scanr_step, scanr_reduce_q]
+        rw [ih]
 
-  lemma scanr_foldr_cons (p: Word α) (q: M.Q) (tail: List β):
-      (p.foldr M.scanr_step (q, tail)).snd = (M.scanr_q p q) ++ tail := by
-    induction p generalizing q tail with
-    | nil =>
-      simp [scanr_q]
-    | cons a p' ih =>
-      simp [scanr_q, scanr_step]
+    lemma scanr_foldr_cons (p: Word α) (q: M.Q) (tail: List β):
+        (p.foldr M.scanr_step (q, tail)).snd = (M.scanr_q q p) ++ tail := by
+      induction p generalizing q tail with
+      | nil =>
+        simp [scanr_q]
+      | cons a p' ih =>
+        simp [scanr_q, scanr_step]
+        rw [scanr_foldr_state]
+        rw [scanr_foldr_state (tail := [])]
+        rw [ih]
+        simp [scanr_q]
+
+    lemma scanr_q_append (p s: Word α) (q: M.Q):
+        M.scanr_q q (p ++ s) = M.scanr_q (M.scanr_reduce_q q s) p ++ M.scanr_q q s := by
+      unfold scanr_q
+      rw [List.foldr_append]
+      let res_s := s.foldr M.scanr_step (q, [])
+      have h_fst : res_s.fst = M.scanr_reduce_q q s := by
+        dsimp [res_s]
+        rw [scanr_foldr_state]
+      have h_snd : res_s.snd = M.scanr_q q s := rfl
+      rw [scanr_foldr_cons]
+      rw [h_fst]
+      rfl
+
+    lemma scanr_append_take (p s: Word α):
+        (M.scanr (p ++ s)).take p.length = M.scanr_q (M.scanr_reduce s) p := by
+      unfold scanr
+      rw [scanr_q_append]
+      apply List.take_left'
+      simp
+
+
+
+
+    @[simp]
+    lemma scanr_reduce_q_empty (q: M.Q): M.scanr_reduce_q q [] = q := by simp [FiniteStateTransducer.scanr_reduce_q]
+
+    @[simp]
+    lemma scanr_reduce_empty: M.scanr_reduce [] = M.q0 := by simp [FiniteStateTransducer.scanr_reduce]
+
+    lemma scanr_reduce_cons (ws: Word α): M.scanr_reduce (w::ws) = M.δ (M.scanr_reduce ws) w := by rfl
+
+
+
+    @[simp]
+    lemma range_of_scanr_q {M: FiniteStateTransducer α β} {q0: M.Q} {w: Word α}: (M.scanr_q q0 w).range = w.range := by
+      simp [Word.range, FiniteStateTransducer.scanr_q_len]
+
+    @[simp]
+    lemma range_of_scanr {M: FiniteStateTransducer α β} {w: Word α}: (M.scanr w).range = w.range := by
+      simp [FiniteStateTransducer.scanr, range_of_scanr_q]
+
+
+
+  /-
+    lemma scanr {M: FiniteStateTransducer α β} (w: Word α) (p: Fin w.length) (q: M.Q):
+        (M.scanr_q q w).get ⟨ p, by simp ⟩ = M.f (M.scanr_reduce_q q (w.drop p)) := sorry
+  -/
+
+
+    lemma scanr_cons (a: α) (w: Word α):
+      M.scanr (a::w) = M.f (M.δ (M.scanr_reduce w) a) :: M.scanr w := by
+      simp [scanr, scanr_q, scanr_step]
       rw [scanr_foldr_state]
-      rw [scanr_foldr_state (tail := [])]
-      rw [ih]
-      simp [scanr_q]
+      rfl
 
-  lemma scanr_q_append (p s: Word α) (q: M.Q):
-      M.scanr_q (p ++ s) q = M.scanr_q p (M.scanr_reduce_q q s) ++ M.scanr_q s q := by
-    unfold scanr_q
-    rw [List.foldr_append]
-    let res_s := s.foldr M.scanr_step (q, [])
-    have h_fst : res_s.fst = M.scanr_reduce_q q s := by
-      dsimp [res_s]
-      rw [scanr_foldr_state]
-    have h_snd : res_s.snd = M.scanr_q s q := rfl
-    rw [scanr_foldr_cons]
-    rw [h_fst]
-    rfl
+    lemma scanr_get'_eq2 (w: Word α) (i: Fin w.length):
+      (M.scanr w)[i]'(by simp) = M.f (M.scanr_reduce w⟦i..*⟧) := by
+      induction w with
+      | nil =>
+        exact i.elim0
+      | cons a w ih =>
+        simp_rw [scanr_cons]
+        match i with
+        | ⟨0, _⟩ =>
+          rfl
+        | ⟨n+1, h⟩ =>
+          simp
+          exact ih ⟨n, Nat.lt_of_succ_lt_succ h⟩
 
-  lemma scanr_append_take (p s: Word α):
-      (M.scanr (p ++ s)).take p.length = M.scanr_q p (M.scanr_reduce s) := by
-    unfold scanr
-    rw [scanr_q_append]
-    apply List.take_left'
-    simp
+    lemma scanr_get'_eq1 (w: Word α) (i: Fin w.length):
+      (M.scanr w)[i]'(by simp) = M.f (M.δ (M.scanr_reduce w⟦i+1..*⟧) w[i]) := by
+      induction w with
+      | nil =>
+        exact i.elim0
+      | cons a w ih =>
+        simp_rw [scanr_cons]
+        match i with
+        | ⟨0, _⟩ =>
+          rfl
+        | ⟨n+1, h⟩ =>
+          simp
+          exact ih ⟨n, Nat.lt_of_succ_lt_succ h⟩
+
+    lemma scanr_get'_eq (w: Word α) (i: ℤ) (h: i ∈ w.range):
+      (M.scanr w).get' i (by simp [h]) = M.f (M.δ (M.scanr_reduce w⟦(i+1).toNat..*⟧) (w.get' i h)) := by
+      rw [Word.get']
+      have h_pos : 0 ≤ i := by simp [Word.range] at h; exact h.1
+      have h_lt : i < w.length := by simp [Word.range] at h; exact h.2
+      have h_nat_lt : i.toNat < w.length := by
+        rwa [Int.toNat_lt h_pos]
+      let idx : Fin w.length := ⟨i.toNat, h_nat_lt⟩
+      have := @scanr_get'_eq1 α β M w idx
+      convert this
+      { grind }
+
+
+
+
+    lemma scanr_reduce_drop (w: Word α) (i: Fin w.length):
+      M.scanr_reduce w⟦i..*⟧ = M.δ (M.scanr_reduce w⟦i+1..*⟧) w[i] := by
+      rw [List.drop_eq_getElem_cons (h := i.isLt)]
+      rw [scanr_reduce_cons]
+      grind
+
+
+    lemma scanr_reduce'? (w: Word α) (i: ℤ):
+      M.scanr_reduce (w.drop i.toNat) = M.δ? (M.scanr_reduce w⟦(i+1).toNat..*⟧) (w.get'? i) := by
+      if h: i ∈ w.range then
+        have h_orig := h
+        rw [Word.range] at h
+        simp only [Set.mem_setOf_eq] at h
+        have h_pos : 0 ≤ i := h.1
+        have h_lt : i < w.length := h.2
+        have h_nat_lt : i.toNat < w.length := by
+          rwa [Int.toNat_lt h_pos]
+        rw [Word.get'?]
+        rw [dif_pos h_orig]
+        rw [List.drop_eq_getElem_cons (h := h_nat_lt)]
+        rw [scanr_reduce_cons]
+        congr
+        . rw [Int.toNat_add h_pos (by decide)]; simp
+      else
+        rw [Word.get'?]
+        rw [dif_neg h]
+        rw [Word.range] at h
+        simp only [Set.mem_setOf_eq] at h
+        if h_neg : i < 0 then
+          have h1 : i.toNat = 0 := Int.toNat_of_nonpos (le_of_lt h_neg)
+          have h2 : (i+1).toNat = 0 := Int.toNat_of_nonpos (by omega)
+          simp [h1, h2, FiniteStateTransducer.δ?]
+        else
+          have h1 : i.toNat ≥ w.length := by omega
+          have h2 : (i+1).toNat ≥ w.length := by omega
+          simp [List.drop_eq_nil_of_le h1]
+          simp [List.drop_eq_nil_of_le h2]
+          simp [FiniteStateTransducer.δ?]
+
+  end
+
+
+  section M_id
+
+    def M_id (α) [Alphabet α]: FiniteStateTransducer α α := {
+      Q := α
+      δ := fun _ a => a
+      q0 := default
+      f := id
+    }
+
+    @[simp]
+    lemma M_id_scanr_eq [Alphabet α]: (M_id α).scanr = id := by
+      funext w
+      simp [FiniteStateTransducer.scanr, FiniteStateTransducer.scanr_q]
+      induction w with
+      | nil => rfl
+      | cons a w ih =>
+        simp [FiniteStateTransducer.scanr_step]
+        rw [ih]
+        cases w <;> simp [M_id]
+
+    @[simp]
+    lemma M_id_advice_eq {α} [Alphabet α]: (M_id α).advice.f = id := by
+      simp [FiniteStateTransducer.advice]
+      rfl
+
+  end M_id
+
+
+  section M_projQ
+
+    def M_projQ (M: FiniteStateTransducer α β): FiniteStateTransducer α M.Q := {
+      Q := M.Q
+      δ := M.δ
+      q0 := M.q0
+      f := id
+    }
+
+
+    lemma M_projQ_scanr (i: ℕ) (h: i < w.length): ((M_projQ M).scanr w)[i]'(by simp_all) = M.scanr_reduce w⟦i..*⟧ := by
+      convert scanr_get'_eq2 (M := M_projQ M) w ⟨i, h⟩
+      simp [M_projQ]
+      generalize w⟦i..*⟧ = w'
+      induction w' with
+      | nil => simp
+      | cons a w' ih =>
+        simp [scanr_reduce_cons]
+        rw [ih]
+
+    @[simp]
+    lemma M_projQ_scanr2: (M_projQ M).scanr w = w.mapIdx fun i _ => M.scanr_reduce w⟦i..*⟧ := by
+      apply List.ext_get
+      · simp
+      intro i h1 h2
+      simp
+      rw [←M_projQ_scanr i]
+      simp_all
+
+  end M_projQ
+
+
+  section M_map
+
+    def M_map [Alphabet α] [Alphabet β] (f: α → β): FiniteStateTransducer α β := (M_id α).map_output f
+
+    @[simp]
+    lemma M_map_scanr [Alphabet α] [Alphabet β] (f: α → β): (M_map f).scanr = List.map f := by
+      simp [M_map, FiniteStateTransducer.map_output_spec, M_id_scanr_eq]
+
+  end M_map
+
+
+  section M_prod
+
+
+    def M_prod [Alphabet α] (M1: FiniteStateTransducer α β1) (M2: FiniteStateTransducer α β2):
+        FiniteStateTransducer α (β1 × β2) :=
+      {
+        Q := M1.Q × M2.Q
+        δ := fun (m_q, c_q) a => (M1.δ m_q a, M2.δ c_q a)
+        q0 := (M1.q0, M2.q0)
+        f := fun (m_q, c_q) => (M1.f m_q, M2.f c_q)
+      }
+
+    private lemma m_prod_scanr_reduce_q [Alphabet α] {M1: FiniteStateTransducer α β1} {M2: FiniteStateTransducer α β2}
+        (q1: M1.Q) (q2: M2.Q) (w: Word α):
+        (M_prod M1 M2).scanr_reduce_q (q1, q2) w = (M1.scanr_reduce_q q1 w, M2.scanr_reduce_q q2 w) := by
+      induction w with
+      | nil => simp [scanr_reduce_q]
+      | cons a w ih =>
+        simp only [scanr_reduce_q]
+        rw [ih]
+        simp [M_prod]
+
+    @[simp]
+    lemma M_prod_spec [Alphabet α] {M1: FiniteStateTransducer α β1} {M2: FiniteStateTransducer α β2}:
+        (M_prod M1 M2).scanr = fun w => List.zip (M1.scanr w) (M2.scanr w) := by
+      funext M2X
+      induction M2X with
+      | nil => simp [scanr, scanr_q]
+      | cons a w ih =>
+        simp only [scanr_cons]
+        rw [ih]
+        simp only [scanr_reduce]
+        rw [show (M_prod M1 M2).q0 = (M1.q0, M2.q0) from rfl]
+        rw [m_prod_scanr_reduce_q]
+        simp [M_prod]
+
+  end M_prod
+
+
+  def comp (M2: FiniteStateTransducer β γ) (M1: FiniteStateTransducer α β): FiniteStateTransducer α γ := {
+    Q := M1.Q × M2.Q
+    δ := fun (q1, q2) a => (M1.δ q1 a, M2.δ q2 (M1.f (M1.δ q1 a)))
+    q0 := (M1.q0, M2.q0)
+    f := fun (_q1, q2) => M2.f q2
+  }
+
+  infixr:90 " ⊚ "  => comp
+
+  @[simp]
+  theorem compose_spec2 [Alphabet α] [Alphabet β] [Alphabet γ]
+    (M2: FiniteStateTransducer β γ) (M1: FiniteStateTransducer α β):
+      (M2 ⊚ M1).scanr = M2.scanr ∘ M1.scanr := by
+    sorry
+
+  theorem compose_spec [Alphabet α] [Alphabet β] [Alphabet γ]
+    (M1: FiniteStateTransducer β γ) (M2: FiniteStateTransducer α β):
+      (M1 ⊚ M2).advice.f = M1.advice.f ∘ M2.advice.f := by
+    sorry
+
+
 
 end FiniteStateTransducer
