CellularAutomatas/proofs/find_some.lean
@@ -1,0 +1,8 @@
+import CellularAutomatas.defs
+
+@[simp]
+lemma apply_iterated_zero {α: Type u} {m: α} {f: α -> α}: apply_iterated f m 0 = m := by
+  simp [apply_iterated]
+
+lemma apply_iterated_succ_apply' {α: Type u} {m: α} {f: α -> α}: apply_iterated f m (n+1) = f (apply_iterated f m n) := by
+  simp [apply_iterated, Function.iterate_succ_apply']
